generator finally working

formic_site_duct/obj/Debug/net6.0/Demo1.AssemblyInfo.cs
@@ -13,7 +13,7 @@ using System.Reflection;
 [assembly: System.Reflection.AssemblyCompanyAttribute("Demo1")]
 [assembly: System.Reflection.AssemblyConfigurationAttribute("Debug")]
 [assembly: System.Reflection.AssemblyFileVersionAttribute("1.0.0.0")]
-[assembly: System.Reflection.AssemblyInformationalVersionAttribute("1.0.0+9c8e1889f4ba82b93afef6e68f7930cc6a4cfa33")]
+[assembly: System.Reflection.AssemblyInformationalVersionAttribute("1.0.0+539b3de00a3bfa4d832e7bd7c52ee65971c5b84d")]
 [assembly: System.Reflection.AssemblyProductAttribute("Demo1")]
 [assembly: System.Reflection.AssemblyTitleAttribute("Demo1")]
 [assembly: System.Reflection.AssemblyVersionAttribute("1.0.0.0")]
